src/Spec/WeakestPreconditions.v
@@ -133,3 +133,6 @@ Section Dynamics.
   Qed.
 
 End Dynamics.
+
+Arguments precondition State T : clear implicits.
+Arguments crashpre State : clear implicits.
